src/specs/PointMulIntoDest.ec
@@ -28,6 +28,15 @@ module PointMulIntoDest = {
       RevertWithMessage.low(W256.of_int 30, W256.zero);
     }
   }
+
+  proc mid(x : int, y : int, s : int) : (int * int) option =
+  {
+    var x_F, y_F, result;
+    x_F <- ZModField.inzmod x;
+    y_F <- ZModField.inzmod y;
+    result <- ecMul_precompile x_F y_F s;
+    return (omap F_to_int_point result);
+  }
 }.
 
 lemma pointMulIntoDest_extracted_equiv_low : equiv [
@@ -41,3 +50,155 @@ proof.
   inline*. wp. skip. by progress.
   inline*. wp. skip. by progress.
 qed.
+
+
+lemma PointAddIntoDest_mid_of_low (x1v y1v sv : int) (p1u destu : uint256) (memory0 : MemoryMap.mem) : equiv [
+    PointMulIntoDest.low ~ PointMulIntoDest.mid :
+    Primops.memory{1} = memory0 /\
+      0 <= x1v < p /\ 0 <= y1v < p /\ 0 <= sv < W256.modulus /\
+      (of_int 128)%W256 <= p1u /\
+      (of_int 128)%W256 <= -p1u /\
+      (of_int 128)%W256 <= p1u + (of_int 32)%W256 /\
+      (of_int 128)%W256 <= - (p1u + (of_int 32)%W256) /\
+    PurePrimops.mload memory0 p1u = W256.of_int x1v /\
+    PurePrimops.mload memory0 (p1u + W256.of_int 32) = W256.of_int y1v /\
+      arg{1} = (p1u, W256.of_int sv, destu) /\ arg{2} = (x1v, y1v, sv) /\ !Primops.reverted{1}
+      ==>
+        exists (memory_F : MemoryMap.mem),
+      memory_F = PurePrimops.mstore (PurePrimops.mstore (PurePrimops.mstore memory0 W256.zero (W256.of_int x1v)) (W256.of_int 32) (W256.of_int y1v)) (W256.of_int 64) (W256.of_int sv)  /\
+      (
+        ConcretePrimops.staticcall_ec_mul_should_succeed (W256.of_int x1v, W256.of_int y1v) (W256.of_int sv) /\
+        exists (x y : F),
+        ecMul_precompile (ZModField.inzmod x1v) (ZModField.inzmod y1v) sv = Some (x, y) /\
+        res{2} = Some (ZModField.asint x, ZModField.asint y) /\
+        Primops.memory{1} = PurePrimops.mstore (PurePrimops.mstore memory_F destu (W256.of_int (ZModField.asint x))) (destu + W256.of_int 32) (W256.of_int (ZModField.asint y)) /\
+        !Primops.reverted{1}
+      ) \/
+      (
+        !ConcretePrimops.staticcall_ec_mul_should_succeed (W256.of_int x1v, W256.of_int y1v) (W256.of_int sv) /\
+        res{2} = None /\
+        Primops.reverted{1}
+      )
+    ]. proof.
+        proc.
+        seq 6 2 :
+    (
+      Primops.memory{1} = PurePrimops.mstore (PurePrimops.mstore (PurePrimops.mstore memory0 W256.zero (W256.of_int x1v)) (W256.of_int 32) (W256.of_int y1v)) (W256.of_int 64) (W256.of_int sv) /\
+      0 <= x1v < p /\ 0 <= y1v < p /\ 0 <= sv < W256.modulus /\
+      (point{1}, s{1}, dest{1}) = (p1u, (of_int sv)%W256, destu) /\
+      (x{2}, y{2}, s{2}) = (x1v, y1v, sv) /\ !Primops.reverted{1} /\
+      x_F{2} = ZModField.inzmod x1v /\ y_F{2} = ZModField.inzmod y1v
+    ).
+        inline *. wp. skip. progress.
+
+        rewrite MemoryMap.load_store_diff. rewrite uint256_sub_zero_eq.
+        apply (uint256_le_le_trans _ (W256.of_int 128) _). smt (@UInt256). exact H7.
+        rewrite uint256_zero_sub_eq_sub. apply (uint256_le_le_trans _ (W256.of_int 128) _). smt (@UInt256). exact H8. rewrite H9 H10. reflexivity.
+
+        case (ConcretePrimops.staticcall_ec_mul_should_succeed (W256.of_int x1v, W256.of_int y1v) (W256.of_int sv)).
+        exists* Primops.memory{1}.
+        elim*=> memory_F.
+        seq 1 1 : 
+    (
+      0 <= x1v < p /\ 0 <= y1v < p /\ 0 <= sv < W256.modulus /\
+      (ConcretePrimops.staticcall_ec_mul_should_succeed (W256.of_int x1v, W256.of_int y1v) (W256.of_int sv)) /\
+      memory_F = PurePrimops.mstore (PurePrimops.mstore (PurePrimops.mstore memory0 W256.zero (W256.of_int x1v)) (W256.of_int 32) (W256.of_int y1v)) (W256.of_int 64) (W256.of_int sv) /\
+        exists (x' y' : F),
+        EllipticCurve.ecMul_precompile (ZModField.inzmod x1v) (ZModField.inzmod y1v) sv = Some (x', y') /\
+        Primops.memory{1} = PurePrimops.mstore (PurePrimops.mstore memory_F destu (W256.of_int (ZModField.asint x'))) (destu + W256.of_int 32) (W256.of_int (ZModField.asint y')) /\
+        result{2} = Some (x',y') /\ 
+        (point{1}, s{1}, dest{1}) = (p1u, (of_int sv)%W256, destu) /\
+        (x{2}, y{2}, s{2}) = (x1v, y1v, sv) /\ !Primops.reverted{1} /\ _10{1} = W256.one /\
+        x_F{2} = ZModField.inzmod x1v /\ y_F{2} = ZModField.inzmod y1v
+      ).
+
+          call {1} (ConcretePrimops.staticcall_ec_mul_pspec memory_F (W256.of_int x1v, W256.of_int y1v) (W256.of_int sv) W256.zero destu).
+      wp. skip. progress. 
+      
+          rewrite MemoryMap.load_store_diff. smt (@W256). smt (@W256).
+          rewrite MemoryMap.load_store_diff. smt (@W256). smt (@W256).
+          rewrite MemoryMap.load_store_same. reflexivity.
+
+          rewrite MemoryMap.load_store_diff. smt (@W256). smt (@W256).
+          rewrite MemoryMap.load_store_same. reflexivity.
+
+          rewrite MemoryMap.load_store_same. reflexivity.
+
+          have J : exists (p : F * F), EllipticCurve.ecMul_precompile
+      ((ZModField.inzmod (to_uint ((of_int x{2})%W256, (of_int y{2})%W256).`1)))
+      ((ZModField.inzmod (to_uint ((of_int x{2})%W256, (of_int y{2})%W256).`2)))
+      (W256.to_uint (W256.of_int s{2}))
+      = Some p. apply exists_of_is_some. smt ().
+        case J.
+      move=> pt.
+        pose x' := pt.`1.
+        pose y' := pt.`2.
+        progress. exists x'. exists y'.
+        progress. have EQ : Some (x', y') = Some pt. smt (). rewrite EQ -H12. congr.
+        rewrite W256.to_uint_small. progress. 
+        apply (lt_trans _ p _). exact H0. exact p_lt_W256_mod.
+        reflexivity.
+        rewrite W256.to_uint_small. progress.
+        apply (lt_trans _ p _). exact H2. exact p_lt_W256_mod.
+        reflexivity.
+        rewrite W256.to_uint_small. progress.
+        reflexivity.
+        smt ().
+        have EQ : Some (x', y') = Some pt. smt (). rewrite EQ -H12. congr.
+        rewrite W256.to_uint_small. progress. 
+        apply (lt_trans _ p _). exact H0. exact p_lt_W256_mod.
+        reflexivity.
+        rewrite W256.to_uint_small. progress. 
+        apply (lt_trans _ p _). exact H2. exact p_lt_W256_mod.
+        reflexivity.
+        rewrite W256.to_uint_small. progress. 
+        reflexivity.
+        smt ().
+
+        rcondf {1} 1. progress. skip. progress. smt (). skip. progress.
+      exists ((PurePrimops.mstore
+     ((PurePrimops.mstore ((PurePrimops.mstore memory0 W256.zero ((of_int x{2}))%W256))
+         ((W256.of_int 32)) ((W256.of_int y{2}))))
+     ((W256.of_int 64)) ((W256.of_int s{2})))).
+       progress. exists x'. exists y'. progress.
+       exists* Primops.memory{1}.
+       elim*=> memory_F.
+       seq 1 1 :
+ (
+   !ConcretePrimops.staticcall_ec_mul_should_succeed (W256.of_int x1v, W256.of_int y1v) (W256.of_int sv) /\ result{2} = None /\ _10{1} = W256.zero
+ ).
+       
+     call {1} (ConcretePrimops.staticcall_ec_mul_pspec memory_F (W256.of_int x1v, W256.of_int y1v) (W256.of_int sv) W256.zero destu).
+     wp. skip. progress.
+
+     rewrite MemoryMap.load_store_diff. smt (@W256). smt (@W256).
+     rewrite MemoryMap.load_store_diff. smt (@W256). smt (@W256).
+     rewrite MemoryMap.load_store_same. reflexivity.
+
+     rewrite MemoryMap.load_store_diff. smt (@W256). smt (@W256).
+     rewrite MemoryMap.load_store_same. reflexivity.
+
+     rewrite MemoryMap.load_store_same. reflexivity.
+
+     have tmp  : (W256.of_int x{2}, W256.of_int y{2}).`1 = W256.of_int x{2}. smt ().
+     have tmp' : (W256.of_int x{2}, W256.of_int y{2}).`2 = W256.of_int y{2}. smt ().
+     have H12 := ConcretePrimops.ecMul_precomp_is_none_of_should_not_succeed (W256.of_int x{2}, W256.of_int y{2}) (W256.of_int s{2}).
+     rewrite tmp tmp' in H12.
+     rewrite to_uint_small in H12. progress. apply (lt_trans _ p _). exact H0. exact p_lt_W256_mod.
+     rewrite to_uint_small in H12. progress. apply (lt_trans _ p _). exact H2. exact p_lt_W256_mod.
+     rewrite to_uint_small in H12. progress.
+
+     apply eq_none_of_is_none.
+ 
+     apply H12.
+
+     progress.
+
+     smt ().
+ 
+     rcondt {1} 1.
+     progress. skip. progress. smt.
+     inline *. wp. skip. progress.
+qed.
+
+      
